intermediate update

src/Example6.v
@@ -27,7 +27,7 @@ Definition v_cons {A : Set} (v : Value A) (l : Label) : Value A :=
   )%string.
 
 (* cons as a function *)
-Definition f_cons : Expr string :=
+Definition f_cons : Value string :=
   (
     [-\] "x",
       [-\] "xs",
@@ -52,10 +52,10 @@ Definition v_of_list {A : Set} (xs : list (Value A)) : Value A * Map A :=
     (v_nil, nil)
     xs.
 
-Fixpoint of_list (l : list (Value string)) : Expr string :=
+Fixpoint e_of_list (l : list (Value string)) : Expr string :=
   match l with
   | []%list => v_nil
-  | (x::xs)%list => f_cons <* x <* Ref (of_list xs)
+  | (x::xs)%list => f_cons <* x <* Ref (e_of_list xs)
   end.
 
 Lemma is_list_update (A : Set) (v : Value A) (m : Map A) l v' :
@@ -123,3 +123,191 @@ Proof.
   - constructor 1.
   - auto using is_list_cons_map, new_label_is_fresh.
 Qed.
+
+Fact f_cons_app_expr :
+  forall (e : Expr _) (v vl : Value _) (m m' m'' : Map _) c c',
+    C[e, m ~~> v, m' | c] ->
+    C[f_cons <* v, m' ~~> vl, m'' | c'] ->
+    C[f_cons <* e, m ~~> vl, m'' | c + c'].
+Proof.
+  eauto using cost_red_comp, cost_red_app2.
+Qed.
+
+Fact f_cons_app_expr2 :
+  forall (e el : Expr _) (v vl vl' : Value _) (m m' m'' m''' : Map _) c c' c'',
+    Is_Valid_Map m ->
+    C[e, m ~~> v, m' | c] ->
+    C[el, m' ~~> vl, m'' | c'] ->
+    C[f_cons <* v <* vl, m'' ~~> vl', m''' | c''] ->
+    exists c''', C[f_cons <* e <* el, m ~~> vl', m''' | c'''].
+Proof.
+  intros e el v vl vl' m m' m'' m''' c c' c'' Hvalid Hred1 Hred2 Hred3.
+  eassert (forall m0, C[f_cons <* v, m0 ~~> _, m0 | 1]) as Hred.
+  { econstructor 2; cbn; econstructor. }
+  cbn in *. remember (-\ RecV [Int 1; shift_v v; Var None]) as vl'' eqn:Hvl''.
+  assert (C[f_cons <* e, m ~~> vl'', m' | c + 1]) as Hred'.
+  { subst. eapply f_cons_app_expr; eauto. }
+  eassert (forall m0, C[ vl'' <* vl, m0 ~~> _, m0 | 1]) as Hred''.
+  { subst. econstructor 2; cbn; econstructor. }
+  cbn in *.
+  remember (RecV [Int 1; bind_v (inc_fun Var vl) (shift_v v); vl])
+    as vl''' eqn:Hvl'''.
+  assert (C[f_cons <* e <* el, m ~~> vl'' <* vl, m'' | (c + 1) + c'])
+    as Hred'''.
+  { eapply cost_red_comp.
+    + eapply cost_red_app1. eassumption.
+    + eapply cost_red_app2. eassumption. }
+  assert (C[f_cons <* e <* el, m ~~> vl''', m'' | ((c + 1) + c') + 1])
+    as Hred''''.
+  { eapply cost_red_comp; eauto. }
+  assert (forall m0, C[f_cons <* v <* vl, m0 ~~> vl'' <* vl, m0 | 1])
+    as Hred'''''.
+  { subst. econstructor 2; repeat econstructor. }
+  assert (forall m0, C[f_cons <* v <* vl, m0 ~~> vl''', m0 | 2])
+    as Hred''''''.
+  { subst. econstructor 2; repeat econstructor. }
+  assert (Is_Valid_Map m') as Hvalid'.
+  { edestruct uniqueness_full as [? [? ?]].
+    + eassumption.
+    + apply Hred1.
+    + eassumption.
+    + assumption. }
+  assert (Is_Valid_Map m'') as Hvalid''.
+  { edestruct uniqueness_full as [? [? ?]].
+    + eassumption.
+    + apply Hred2.
+    + eassumption.
+    + assumption. }
+  destruct (uniqueness_full _ _ _ _ _ _ _ _ _ Hvalid'' Hred3 (Hred'''''' m''))
+    as [? [? ?]].
+  subst. eauto.
+Qed.
+
+(* goal 3 *)
+Lemma f_cons_red_to_list :
+  forall (e el : Expr _) l (v vl vl' : Value _) (m m' m'' m''' m'''' : Map _)
+    c c' c'' c''',
+    Is_Valid_Map m ->
+    C[e, m ~~> v, m' | c] ->
+    C[el, m' ~~> vl, m'' | c'] ->
+    C[Ref vl, m'' ~~> Lab l, m''' | c''] ->
+    C[f_cons <* e <* Ref el, m ~~> vl', m'''' | c'''] ->
+    is_list vl m'' ->
+    is_list vl' m''''.
+Proof.
+  intros e el l v vl vl' m m' m'' m''' m'''' c c' c'' c'''
+    Hvalid Hred Hred1 Hred2 Hred3 His_list.
+  assert (Is_Valid_Map m') as Hvalid'.
+  { edestruct uniqueness_full as [? [? ?]].
+    + eassumption.
+    + apply Hred.
+    + eassumption.
+    + assumption. }
+  assert (Is_Valid_Map m'') as Hvalid''.
+  { edestruct uniqueness_full as [? [? ?]].
+    + eassumption.
+    + apply Hred1.
+    + eassumption.
+    + assumption. }
+  eassert (C[Ref el, m' ~~> Lab l, m''' | c' + c'']) as Hred'.
+  { eapply cost_red_comp.
+    + eapply cost_red_ref_e. eassumption.
+    + eassumption. }
+  eassert (Lookup l m''' vl /\ is_list vl m''') as [Hlookup His_list'].
+  { inversion Hred2. subst. inversion H; try discriminate_red_Val.
+    subst. inversion H0; try discriminate_red_Val. subst. split.
+    + constructor.
+    + apply is_list_cons_map.
+      * apply new_label_is_fresh.
+      * assumption. }
+  eassert (forall m0, C[f_cons <* v <* vl, m0 ~~> _, m0 | 2])
+    as Hred''.
+  { econstructor.
+    + repeat econstructor.
+    + cbn. econstructor.
+      * econstructor.
+      * cbn. econstructor. }
+  remember (RecV [Int 1; bind_v (inc_fun Var vl) (shift_v v); vl]) as v'
+    eqn:Hv'.
+  specialize Hred'' with m''' as Hred'''.
+  edestruct f_cons_app_expr2 as [c'''' Hred''''].
+  - eapply Hvalid.
+  - eapply Hred.
+  - eapply Hred'.
+  - econstructor 2.
+    + repeat econstructor.
+    + cbn. econstructor 2.
+      * repeat econstructor.
+      * cbn. econstructor.
+  - destruct (uniqueness_full _ _ _ _ _ _ _ _ _ Hvalid Hred3 Hred'''')
+      as [? [? ?]].
+    subst. econstructor; eauto.
+Qed.
+
+Lemma e_of_list_v_of_list :
+  forall xs v m, exists c,
+    v_of_list xs = (v, m) ->
+    C[e_of_list xs, nil ~~> v, m | c].
+Proof.
+  induction xs; simpl.
+  - intros v m. eexists. intros Heq. injection Heq as [] []. constructor.
+  - intros v m. destruct v_of_list. destruct (IHxs v0 m0). eexists. intros Heq.
+    injection Heq as [] []. eapply cost_red_comp.
+    + eapply cost_red_app1. econstructor 2.
+      * econstructor.
+      * cbn. econstructor.
+    + eapply cost_red_comp.
+      * eapply cost_red_app2, cost_red_ref_e. auto.
+      * econstructor 2.
+        -- eapply red_app2. econstructor. reflexivity.
+        -- econstructor 2.
+          ++ econstructor.
+          ++ cbn. unfold v_cons. admit. (* econstructor 1.*)
+Admitted.
+
+(* goal 4 *)
+Lemma e_of_list_is_list :
+  forall xs (v : Value _) (m m' : Map _) c,
+    Is_Valid_Map m ->
+    C[e_of_list xs, m ~~> v, m' | c] ->
+    is_list v m'.
+Proof.
+  intros xs v m m' c Hvalid Hred.
+  destruct (v_of_list xs) eqn:Hxs.
+  destruct e_of_list_v_of_list with xs v0 m0. specialize (H Hxs).
+  eapply extend_state in H.
+  - inversion Hred; [constructor | discriminate_red_Val].
+  - eapply f_cons_red_to_list.
+(*
+  induction xs; simpl; intros v m m' c Hvalid Hred.
+  - inversion Hred; [constructor | discriminate_red_Val].
+  - eapply f_cons_red_to_list.
+    + eassumption.
+    + econstructor 1.
+    +
+  
+   inversion Hred; subst.
+    repeat match goal with
+    | [H : red _ _ _ _ |- _] =>
+      inversion H; subst; cbn in *; clear H
+    end.
+    inversion H0; subst.
+    inversion H; subst; cbn in *; clear H; try discriminate_red_Val.
+    destruct xs; simpl in *.
+    inversion H7; subst; cbn in *; clear H7.
+    + unfold e_of_list in H. destruct xs; try discriminate.
+      injection H. intro. subst. simpl in *. eapply IHxs.
+        .
+    repeat match goal with
+    | [H : red _ _ _ _ |- _] =>
+      inversion H; subst; cbn in *; clear H
+    end.
+   eapply f_cons_is_list.
+    + exact Hred. eassumption.
+   destruct v_of_list. injection Heq as [] [].
+    econstructor.
+    + apply Lookup_spec_eq. apply lookup_same.
+    + apply is_list_update; auto. apply new_label_is_fresh.
+Qed.
+*)
+Admitted.
